stuff

proofs/Challenge2_proof.v
@@ -15,7 +15,7 @@ Open Scope Z_scope.
 
 Hint Constructors LocallySorted.
 Hint Constructors Permutation.
-Ltac auto_tilde ::= try unfold LibListZ.length in *; rew_list in *; eauto with maths.
+Ltac auto_tilde ::= (* try unfold LibListZ.length in *;  *)rew_list in *; eauto with maths.
 
 Inductive color := R | B.
 Definition coloring := list color.
@@ -29,18 +29,93 @@ Fixpoint coloring_valid (aux: int) (c : coloring) : bool :=
   | nil => if Z_lt_le_dec aux 3 then false else true
   end.
 
-Definition invariant (n: int) (counts: list int) (colorings: list coloring) :=
+Definition invariant (n: int) (counts: list int) (colorings: list (list coloring)) :=
   length counts = n /\
   length colorings = n /\
   forall i, 0 <= i < n ->
     counts[i] = length colorings[i] /\
-    Forall (fun c => length c = i) colorings.
+    Forall (fun c => length c = i) colorings[i].
 
-Lemma docount_spec : forall (a:loc) (L: list int),
-  app docount [count a]
+Lemma docount_spec : forall (a: array int) (L: list int),
+  length L >= 4 ->
+  app docount [a]
     PRE (a ~> Array L)
     POST (fun (tt:unit) =>
             Hexists L' C,
             a ~> Array L' \* \[ invariant (length L') L' C ]).
 Proof.
-Admitted.
+  introv. xcf.
+  xapps. xapps. { apply~ index_of_inbound.  }
+  xapps. { apply~ index_of_inbound. rewrite length_update. math. }
+  xapps. { apply~ index_of_inbound. rewrite !length_update. math. }
+  xapps. { apply~ index_of_inbound. rewrite !length_update. math. }
+  xfor_inv (fun n => Hexists L0 Ljunk C,
+                     a ~> Array (L0 ++ Ljunk) \*
+                     \[ length L0 = n /\
+                        length L0 + length Ljunk = length L /\
+                        invariant n L0 C ]).
+  { math. }
+  { do 4 (destruct L as [|? L];  try solve [ false~ ]).
+    hsimpl (>> (1 :: 1 :: 1 :: 2 :: nil) L
+               ((nil :: nil) :: ((B :: nil) :: nil) :: ((B :: B :: nil) :: nil) ::
+                             ((B::B::B::nil) :: (R::R::R::nil) :: nil) :: nil)).
+    rew_list. rewrite update_zero. rewrite~ update_cons_pos.
+    rewrite update_zero. repeat (try rewrite update_zero; rewrite~ update_cons_pos).
+    repeat f_equal. rewrite update_zero. f_equal.
+    splits~. unfolds~ invariant. splits~.
+    { intros i Hi.
+      admit. } }
+  { intros n (Hilo & Hihi).
+    xpull. intros L0 Ljunk C (? & (I1 & I2)).
+    xapps. { apply~ index_of_inbound. }
+    xapps. { apply~ index_of_inbound. }
+    destruct Ljunk as [| ? Ljunk']. { false~. math. }
+    rewrite update_middle with (l1 := L0) (l2 := Ljunk'); [| auto_tilde].
+    rew_list in I1.
+    pose (C' := map (cons B) C[n-1]).
+    assert ((L0 ++ z :: Ljunk')[n-1] = L0[n-1]) as ->.
+    { rewrite read_app. case_if~. }
+    xfor_inv (fun (k:int) =>
+      Hexists (count: int) (C': list coloring),
+        a ~> Array (L0 ++ count :: Ljunk') \*
+        \[ count = length C' /\
+           Forall (fun c => length c = n) C'
+        ]).
+    { math. }
+    { hsimpl L0[n-1] C'.
+      { rew_list. reflexivity. }
+      { splits~.
+        - unfold invariant in I2. unpack.
+          subst C'. rewrite length_map. apply~ H3.
+        - unfold invariant in I2. unpack.
+          subst C'.
+          forwards~: H3 (n-1). unpack.
+
+          Lemma Forall_map {A B : Type} { P : B -> Prop} {f : A -> B} {l: list A} :
+            Forall (fun x => P (f x)) l ->
+            Forall P (map f l).
+          Proof. induction 1; now constructor. Qed.
+          apply Forall_map.
+
+          apply (Forall_pred_incl H5). unfold pred_incl.
+          intros. auto_tilde. } }
+    { intros k (Hk1 & Hk2). xpull. intros count C'0 (II1 & II2).
+      xapps. { apply~ index_of_inbound. }
+      xapps. { apply~ index_of_inbound. }
+      xapps. { apply~ index_of_inbound. }
+      hsimpl
+        (count + L0[n-k-1])
+        ((map (fun c => ((make k R) ++ B :: c)) C[n-k-1]) ++ C'0).
+      { rewrite read_middle with (x := count); [|auto_tilde].
+        rewrite update_middle with (w := count); [| auto_tilde].
+        assert ((L0 ++ count :: Ljunk')[(n-k)-1] = L0[n-k-1]) as ->. {
+          rewrite read_app. case_if~. }
+        rew_list~. }
+      { splits~.
+        { rewrite length_map. unfold invariant in I2. unpack.
+          rewrite II1. forwards~: H3 ((n-k)-1). unpack.
+          rewrite H4. rewrite Z.add_comm. reflexivity. }
+        { admit. } } }
+    { admit. } }
+  { admit. }
+Qed.
